sep: refactor

bedrock2/src/Map.v
@@ -9,6 +9,15 @@ Module map.
   }.
   Arguments map : clear implicits.
 
+  Class ok {key value} (map : map key value) := {
+    map_ext : forall m1 m2, (forall k, get m1 k = get m2 k) -> m1 = m2;
+    get_empty : forall k, get empty k = None;
+    get_put_same : forall m k v, get (put m k v) k = Some v;
+    get_put_diff : forall m k v k', k <> k' -> get (put m k' v) k = get m k;
+    get_union_left : forall m1 m2 k, get m2 k = None -> get (union m1 m2) k = get m1 k;
+    get_union_right : forall m1 m2 k v, get m2 k = Some v -> get (union m1 m2) k = Some v;
+  }.
+
   Section ListOperations.
     Context {key value} {map : map key value}.
     Fixpoint putmany (keys : list key) (values : list value) (m : rep) {struct keys} : option rep :=
@@ -20,32 +29,41 @@ Module map.
       end.
   End ListOperations.
 
+  Section Decomp.
+    Context {key value} {map : map key value}.
+    Definition disjoint (a b : rep) : Prop :=
+      forall k v1 v2, get a k = Some v1 -> get b k = Some v2 -> False.
+    Definition split m m1 m2 : Prop :=
+      m = (union m1 m2) /\ disjoint m1 m2.
+    Definition carve m1 m P2 : Prop :=
+      exists m2, split m m2 m1 /\ P2 m2.
+    Fixpoint splits m ms : Prop :=
+      match ms with
+      | nil => m = empty
+      | cons m0 ms' => carve m0 m (fun m => splits m ms')
+      end.
+  End Decomp.
+
   Require Import Coq.Setoids.Setoid Coq.Classes.Morphisms.
   Section Properties.
     (* FIXME: move proofs to a different file *)
-    Context {key value} {map : map key value}.
-    Context (map_ext : forall m1 m2, (forall k, get m1 k = get m2 k) -> m1 = m2).
-    Context (get_empty : forall k, get empty k = None).
-    Context (union_None : forall m1 m2 k, get m2 k = None -> get (union m1 m2) k = get m1 k).
-    Context (union_Some : forall m1 m2 k v, get m2 k = Some v -> get (union m1 m2) k = Some v).
-    
-    Definition disjoint (a b : rep) : Prop :=
-      forall k v1 v2, get a k = Some v1 -> get b k = Some v2 -> False.
+    Context {key value} {map : map key value} {ok : ok map}.
 
     Lemma union_spec m1 m2 k :
       (exists v, get m2 k = Some v /\ get (union m1 m2) k = Some v) \/
       (get m2 k = None /\ get (union m1 m2) k = get m1 k).
     Proof.
       destruct (get m2 k) eqn:?HH; [left | right ].
-      { exists v. split. reflexivity. erewrite union_Some; eauto. }
-      { split. reflexivity. rewrite union_None; eauto. }
+      { exists v. split. reflexivity. erewrite get_union_right; eauto. }
+      { split. reflexivity. rewrite get_union_left; eauto. }
     Qed.
     
     Lemma union_comm x y : disjoint x y -> union x y = union y x.
     Proof.
       cbv [disjoint]; intros; eapply map_ext; intros.
       destruct (get x k) eqn:Hl, (get y k) eqn:Hr;
-        repeat ((erewrite union_None by eauto) || (erewrite union_Some by eauto));
+        repeat ((erewrite get_union_left by eauto)
+                || (erewrite get_union_right by eauto));
         firstorder congruence.
     Qed.
 
@@ -65,22 +83,12 @@ Module map.
     Qed.
 
     Lemma union_empty_r x : union x empty = x.
-    Proof. eapply map_ext; intros; rewrite union_None; eauto. Qed.
+    Proof. eapply map_ext; intros; rewrite get_union_left; eauto using get_empty. Qed.
     Lemma union_empty_l x : union empty x = x.
-    Proof. rewrite (union_comm empty x) by congruence; eapply union_empty_r. Qed.
-    
-    Definition split m m1 m2 : Prop :=
-      m = (union m1 m2) /\ disjoint m1 m2.
-    Definition carve m1 m P2 : Prop :=
-      exists m2, split m m2 m1 /\ P2 m2.
-    Fixpoint splits m ms : Prop :=
-      match ms with
-      | nil => m = empty
-      | cons m0 ms' => carve m0 m (fun m => splits m ms')
-      end.
+    Proof. rewrite (union_comm empty x); destruct ok; eauto || congruence. Qed.
                               
-    Lemma disjoint_empty_l x : disjoint empty x. repeat intro; congruence. Qed.
-    Lemma disjoint_empty_r x : disjoint x empty. repeat intro; congruence. Qed.
+    Lemma disjoint_empty_l x : disjoint empty x. destruct ok; repeat intro; congruence. Qed.
+    Lemma disjoint_empty_r x : disjoint x empty. destruct ok; repeat intro; congruence. Qed.
     Lemma disjoint_comm m1 m2 : disjoint m1 m2 <-> disjoint m2 m1.
     Proof. cbv [disjoint]. firstorder idtac. Qed.
     Lemma disjoint_union_r x y z : disjoint x (union y z) <-> (disjoint x y /\ disjoint x z).
@@ -135,82 +143,97 @@ Module map.
       cbv [Proper respectful]; intros x y H; revert m; induction H; intros;
         try solve [ eapply carve_comm | firstorder idtac ].
     Qed.
+  End Properties.
 
+  Section Lift1Prop.
     Definition impl1 {T} (P Q:_->Prop) : Prop := forall x:T, P x -> Q x.
+    Definition iff1 {T} (P Q:_->Prop) : Prop := forall x:T, P x <-> Q x.
+    Definition ex1 {A B} (P : A -> B -> Prop) := fun (b:B) => exists a:A, P a b.
     Global Instance Transitive_impl1 T : Transitive (@impl1 T). firstorder idtac. Qed.
     Global Instance Reflexive_impl1 T : Reflexive (@impl1 T). firstorder idtac. Qed.
     Global Instance Proper_impl1_impl1 T : Proper (Basics.flip impl1 ==> impl1 ==> Basics.impl) (@impl1 T). firstorder idtac. Qed.
-    Definition iff1 {T} (P Q:_->Prop) : Prop := forall x:T, P x <-> Q x.
     Global Instance subrelation_iff1_impl1 T : subrelation (@iff1 T) (@impl1 T). firstorder idtac. Qed.
     Global Instance Equivalence_iff1 T : Equivalence (@iff1 T). firstorder idtac. Qed.
     Global Instance Proper_iff1_iff1 T : Proper (iff1 ==> iff1 ==> iff) (@iff1 T). firstorder idtac. Qed.
     Global Instance Proper_iff1_impl1 T : Proper (Basics.flip impl1 ==> impl1 ==> Basics.impl) (@impl1 T). firstorder idtac. Qed.
     Global Instance Proper_impl1_iff1 T : Proper (iff1 ==> iff1 ==> iff) (@impl1 T). firstorder idtac. Qed.
+    Global Instance Proper_ex1_iff1 A B : Proper (pointwise_relation _ iff1 ==> iff1) (@ex1 A B). firstorder idtac. Qed.
+    Global Instance Proper_ex1_impl1 A B : Proper (pointwise_relation _ impl1 ==> impl1) (@ex1 A B). firstorder idtac. Qed.
+    Lemma impl1_ex1_l {A B} p q : impl1 (@ex1 A B p) q <-> (forall x, impl1  (p x) q).
+    Proof. firstorder idtac. Qed.
+    Lemma impl1_ex1_r {A B} p q x : impl1 p (q x) -> impl1 p (@ex1 A B q).
+    Proof. firstorder idtac. Qed.
+  End Lift1Prop.
+
+  Section Sep.
+    Context {key value} {map : map key value}.
     Definition emp (P : Prop) := fun m => m = empty /\ P.
-    Global Instance Proper_emp_iff : Proper (iff ==> iff1) emp. firstorder idtac. Qed.
-    Global Instance Proper_emp_impl : Proper (Basics.impl ==> impl1) emp. firstorder idtac. Qed.
     Definition sep (p q : rep -> Prop) m :=
       exists mp mq, split m mp mq /\ p mp /\ q mq.
+    Definition ptsto k v := fun m => m = put empty k v.
+    Definition read k (P : value -> rep -> Prop) := (ex1 (fun v => sep (ptsto k v) (P v))).
+  End Sep.
+
+  Section SepProperties.
+    Context {key value} {map : map key value} {ok : ok map}.
     Local Infix "*" := sep.
+
+    Global Instance Proper_emp_iff : Proper (iff ==> iff1) emp. firstorder idtac. Qed.
+    Global Instance Proper_emp_impl : Proper (Basics.impl ==> impl1) emp. firstorder idtac. Qed.
     Global Instance Proper_sep_iff1 : Proper (iff1 ==> iff1 ==> iff1) sep. firstorder idtac. Qed.
     Global Instance Proper_sep_impl1 : Proper (impl1 ==> impl1 ==> impl1) sep. firstorder idtac. Qed.
-    Definition ptsto k v := fun m => m = put empty k v.
-    Definition exi {T} (P : T -> rep -> Prop) := fun m => exists x:T, P x m.
-    Global Instance Proper_exi_iff1 T : Proper (pointwise_relation _ iff1 ==> iff1) (@exi T). firstorder idtac. Qed.
-    Global Instance Proper_exi_impl1 T : Proper (pointwise_relation _ impl1 ==> impl1) (@exi T). firstorder idtac. Qed.
-    Definition read k (P : value -> rep -> Prop) := (exi (fun v => ptsto k v * P v)).
-    
 
+    Ltac t :=
+      repeat match goal with
+      | _ => progress subst
+      | H:_ /\ _ |- _ => destruct H
+      | H:exists _, _ |- _ => destruct H
+      | H:disjoint (union _ _) _ |- _ => eapply disjoint_union_l in H; destruct H
+      | H:disjoint _ (union _ _) |- _ => eapply disjoint_union_r in H; destruct H
+      | _ => progress intuition idtac
+      end.
+
+    (* sep and sep *)
     Lemma sep_comm p q : iff1 (p*q) (q*p).
-    Proof. cbv [iff1 sep split]; firstorder (subst; eauto using union_comm). Qed.
+    Proof. cbv [iff1 sep split]; t; eauto 10 using union_comm, (fun m1 m2 => proj2 (disjoint_comm m1 m2)). Qed.
     Lemma sep_assoc p q r : iff1 ((p*q)*r) (p*(q*r)).
-    Proof. cbv [iff1 sep split]; split; t;
-           eauto 15 using eq_sym, union_assoc, ((fun m1 m2 m3 => proj2 (disjoint_union_l m1 m2 m3))), ((fun m1 m2 m3 => proj2 (disjoint_union_r m1 m2 m3))).
-    Qed.
-    Lemma sep_cancel (p1 p2 q1 q2:_->Prop) (_:impl1 p1 p2) (_:impl1 q1 q2) : impl1 (p1*q1) (p2*q2).
-    Proof. cbv [impl1 sep]; firstorder idtac. Qed.
+    Proof. cbv [iff1 sep split]; t; eauto 15 using eq_sym, union_assoc, ((fun m1 m2 m3 => proj2 (disjoint_union_l m1 m2 m3))), ((fun m1 m2 m3 => proj2 (disjoint_union_r m1 m2 m3))). Qed.
+    Lemma sep_213 B A C : iff1 (A * (B * C)) (B * (A * C)).
+    Proof. rewrite <-(sep_assoc _ B), (sep_comm _ B), sep_assoc. reflexivity. Qed.
+
+    (* sep and ex1 *)
+    Lemma sep_ex1_r {T} p (q:T->_) : iff1 (p * ex1 q) (ex1 (fun h => p * q h)).
+    Proof. firstorder idtac. Qed.
+    Lemma sep_ex1_l {T} p (q:T->_) : iff1 (ex1 q * p) (ex1 (fun h => q h * p)).
+    Proof. rewrite sep_comm. rewrite sep_ex1_r. setoid_rewrite (sep_comm p). reflexivity. Qed.
+
+    (* sep and emp *)
     Lemma sep_emp_emp p q : iff1 (sep (emp p) (emp q)) (emp (p /\ q)).
     Proof. cbv [iff1 sep emp split]; t; intuition eauto 20 using union_empty_l, disjoint_empty_l. Qed.
-    Lemma sep_exi_r {T} p q : iff1 (p * @exi T q) (exi (fun h => p * q h)).
-    Proof. cbv [exi sep]; firstorder idtac. Qed.
-    Lemma sep_exi_l {T} p q : iff1 (@exi T q * p) (exi (fun h => q h * p)).
-    Proof. rewrite sep_comm. rewrite sep_exi_r. setoid_rewrite (sep_comm p). reflexivity. Qed.
-    Lemma impl1_exi_l {T} p q : impl1 (exi p) q <-> (forall x:T, impl1 (p x) q).
-    Proof. cbv [exi sep impl1]; firstorder idtac. Qed.
-    Lemma impl1_exi_r {T} p q (x:T) : impl1 p (q x) -> impl1 p (exi q).
-    Proof. cbv [exi sep impl1]; firstorder idtac. Qed.
-
-    Lemma sep_213 B A C : iff1 (A * (B * C)) (B * (A * C)).
-    Proof. rewrite <-(fun a b => sep_assoc a B b), (fun a => sep_comm a B), sep_assoc. reflexivity. Qed.
     Lemma sep_emp_r a b : iff1 (a * emp b) (emp b * a). eapply sep_comm. Qed.
     Lemma sep_emp_2 a b c : iff1 (a * (emp b * c)) (emp b * (a * c)).
     Proof. rewrite <-sep_assoc. rewrite (sep_comm a). rewrite sep_assoc. reflexivity. Qed.
     Lemma sep_emp_12 a b c : iff1 (emp a * (emp b * c)) (emp (a /\ b) * c).
     Proof. rewrite <-sep_assoc. rewrite sep_emp_emp. reflexivity. Qed.
 
+    (* impl1 and emp *)
     Lemma impl1_l_sep_emp (a:Prop) b c : impl1 (emp a * b) c <-> (a -> impl1 b c).
-    Proof.
-      cbv [impl1 emp sep split]. firstorder idtac; subst; rewrite ?union_empty_l; eauto.
-      eapply H. exists empty, x.  rewrite union_empty_l. repeat split; eauto using disjoint_empty_l.
-    Qed.
-
+    Proof. cbv [impl1 emp sep split]; t; rewrite ?union_empty_l; eauto 10 using union_empty_l, disjoint_empty_l. Qed.
     Lemma impl1_r_sep_emp a b c : (b /\ impl1 a c) -> impl1 a (emp b * c).
-    Proof.
-      cbv [impl1 emp sep split]. firstorder idtac; subst.
-      exists empty, x. rewrite union_empty_l. repeat split; eauto using disjoint_empty_l.
-    Qed.
+    Proof. cbv [impl1 emp sep split]; t; eauto 10 using union_empty_l, disjoint_empty_l. Qed.
 
     Ltac set_evars := repeat match goal with |- context[?e] => is_evar e; set e end.
     Ltac subst_evars := repeat match goal with x := ?e |- _ => is_evar e; subst x end.
     Ltac normalize :=
       set_evars;
-      repeat (rewrite_strat (bottomup (terms @sep_emp_emp @sep_emp_r @sep_emp_12 @sep_emp_2 @sep_exi_l @sep_exi_r @sep_assoc)));
+      (* COQBUG? Why is the repeat necessary? Why does it not work inside rewrite_strat? *)
+      repeat (rewrite_strat (bottomup (terms @sep_emp_emp @sep_emp_r @sep_emp_12 @sep_emp_2 @sep_ex1_l @sep_ex1_r @sep_assoc)));
       subst_evars.
     Ltac cancel_atom_goal1 P :=
       (* COQBUG: if I use fresh here, rewrite_strat fails *)
-      pose proof (sep_213 P) as _cancel_atom_goal1_ASDA;
-      (rewrite_strat (try (bottomup (terms _cancel_atom_goal1_ASDA))));
-      clear _cancel_atom_goal1_ASDA.
+      pose proof (sep_213 P) as __PRIVATE_cancel_atom_goal1_ASDA;
+      (rewrite_strat (try (bottomup (terms __PRIVATE_cancel_atom_goal1_ASDA))));
+      clear __PRIVATE_cancel_atom_goal1_ASDA.
     Ltac cancel_atom P :=
       eapply Proper_impl1_impl1; [ cbv [Basics.flip]; cancel_atom_goal1 P; eapply (Proper_sep_impl1 P _ (reflexivity _)) | reflexivity | reflexivity ].
     Ltac cancel :=
@@ -219,24 +242,25 @@ Module map.
       repeat match goal with |- impl1 _ (?P * _) => cancel_atom P end;
       subst_evars.
 
-    Goal forall A B C D E, exists R, impl1 (A*emp True*B*exi(fun x:unit => C*(exi (fun v : value => (emp (x = x)* emp(v =v))*E v x)))*D) (A * exi (fun n => C * emp (1=n)) * R).
+    Goal forall A B C D E, exists R, impl1 (A*emp True*B*ex1(fun x:unit => C*(ex1 (fun v : value => (emp (x = x)* emp(v =v))*E v x)))*D) (A * ex1 (fun n => C * emp (1=n)) * R).
     Proof.
       intros.
       normalize.
       eexists ?[R].
-      eapply impl1_exi_r.
+      eapply impl1_ex1_r.
       eapply impl1_r_sep_emp.
       split. reflexivity.
-      apply impl1_exi_l. intros.
-      apply impl1_exi_l. intros.
+      apply impl1_ex1_l. intros.
+      apply impl1_ex1_l. intros.
       apply impl1_l_sep_emp. intros.
       cancel.
-      instantiate (1 := exi (fun x0 => exi (fun x => (B * (E x0 x * D))))).
-      eapply impl1_exi_r.
-      eapply impl1_exi_r.
+      (* packaging up the context: *)
+      instantiate (1 := ex1 (fun x0 => ex1 (fun x => (B * (E x0 x * D))))).
+      eapply impl1_ex1_r.
+      eapply impl1_ex1_r.
       reflexivity.
     Qed.
-  End Properties.
+  End SepProperties.
   
 End map. Notation map := map.map.
 Global Coercion map.rep : map >-> Sortclass.
